moved most of dequeuer ghost theory to a separate file

lawyer/nonblocking/examples/queue/dequeuer/dequeue.v
@@ -9,360 +9,11 @@ From lawyer Require Import sub_action_em program_logic.
 From iris.algebra Require Import auth gmap gset excl excl_auth csum mono_nat.
 From iris.base_logic.lib Require Import invariants.
 From lawyer.nonblocking.examples.queue Require Import simple_queue_utils simple_queue.
-From lawyer.nonblocking.examples.queue.dequeuer Require Import dequeuer_lib.
+From lawyer.nonblocking.examples.queue.dequeuer Require Import dequeuer_lib dequeue_ghost.
 From heap_lang Require Import heap_lang_defs lang notation.
 
 
 Close Scope Z.
-
-
-Section DequeueGhost.
-  Context {Σ} {hG: heap1GS Σ} {iG: invGS_gen HasNoLc Σ}.  
-  Context {QL: QueueG Σ}.
-  
-  (* TODO: move *)
-  Lemma is_LL_into_drop hq pt k
-    (LL: is_LL_into hq pt):
-    is_LL_into (drop k hq) pt.
-  Proof using.
-    revert k. induction hq.
-    { intros. by rewrite drop_nil. }
-    intros. destruct k.
-    { by rewrite drop_0. }
-    simpl. apply IHhq.
-    simpl in LL. destruct a as [? [? ?]].
-    destruct hq; try done.
-    destruct h as [? [? ?]]. tauto.
-  Qed.
-
-  (* TODO: move *)
-  Lemma dom_max_set_fold n:
-    set_fold max 0 (set_seq 0 (S n): gset nat) = n.
-  Proof using.
-    clear. induction n.
-    { done. }
-    rewrite set_seq_S_end_union_L.
-    rewrite union_comm_L. 
-    erewrite set_fold_union.
-    2-4: red; lia.
-    simpl. rewrite IHn.
-    rewrite set_fold_singleton. lia.
-  Qed.
-
-  Definition upd_rp rp :=
-    match rp with
-    | rs_init => rs_canceled
-    | rs_proc (Some rsp_going) => rs_proc (Some rsp_protected)
-    | _ => rp
-    end. 
-
-  Lemma upd_rp_rs_step p: rs_step p (upd_rp p).
-  Proof using.
-    destruct p; simpl; try constructor.
-    destruct orsp; simpl; try constructor.
-    destruct r; repeat constructor.
-  Qed.
-
-  Lemma read_hist_wf_bump (hist: read_hist) rop h rp
-    (RH_WF: read_hist_wf hist rop h)
-    (n := set_fold max 0 (dom hist)):
-    read_hist_auth hist -∗ ith_rp n rp ==∗
-    ∃ r rp', let hist' := <[ n := ((r, h + 1), rp') ]> hist in
-      read_hist_auth hist' ∗ ith_read n r (h + 1) ∗ ⌜ read_hist_wf hist' rop (h + 1) ⌝ ∗
-      ith_rp n (upd_rp rp) ∗ ⌜ r <= h ⌝.
-  Proof using.
-    rewrite /read_hist_wf. iIntros "AUTH RP".
-    destruct RH_WF as (n_ & DOM & ROP & SEQ & BB).
-
-    assert (n_ = n) as ->.
-    { subst n. rewrite DOM. by rewrite dom_max_set_fold. }
-
-    destruct (hist !! n) as [[[r b0] p]| ] eqn:NTH.
-    2: { apply not_elem_of_dom in NTH. rewrite DOM in NTH.
-         rewrite elem_of_set_seq in NTH. lia. }
-    iDestruct (ith_rp_hist_compat with "[$] [$]") as %(? & ? & EQ').
-    rewrite NTH in H. inversion H. subst x. simpl in EQ'. clear H.
-    rename rp into p_. 
-    
-    iMod (read_hist_update' _ _ _ _ _ (h + 1) with "AUTH RP") as "(AUTH & #ITH & RP)".
-    { apply upd_rp_rs_step. }
-    { apply NTH. }
-
-    rewrite Nat.max_r.
-    2: { apply BB in NTH. simpl in NTH. lia. }
-    iModIntro. do 2 iExists _. iFrame "AUTH ITH RP".
-    iPureIntro. split.
-    2: { eapply BB in NTH; eauto. by apply NTH. }
-
-    exists n. split; [| split; [| split]]. 
-    - rewrite dom_insert_L. apply mk_is_Some, elem_of_dom in NTH. set_solver.
-    - done.
-    - intros ?????. rewrite !lookup_insert_Some.
-      intros [(? & ?) | (? & ITH) ] [(? & ?) | (? & JTH) ]; subst; simpl in *; try lia.
-      + apply mk_is_Some, elem_of_dom in JTH.
-        rewrite DOM elem_of_union elem_of_set_seq elem_of_singleton in JTH. lia.
-      + eapply SEQ in H; eauto. done.
-      + eapply SEQ; eauto.
-    - intros ??. rewrite lookup_insert_Some.         
-      intros [(? & ?) | (? & ITH) ]; subst; simpl; try lia.
-      { eapply BB in NTH; eauto. simpl in NTH. lia. }
-      eapply BB in ITH; eauto. lia.
-  Qed.
-
-  Lemma upd_rp_fin_pres rs
-    (FIN: rs_fin rs):
-    rs_fin (upd_rp rs).
-  Proof using.
-    red. destruct FIN as [-> | [-> | [-> | ->]]]; subst; simpl; try by eauto.
-  Qed.
-
-  (* TODO: move *)
-  Lemma drop_drop_comm: ∀ {A : Type} (l : list A) (n1 n2 : nat),
-      drop n1 (drop n2 l) = drop n2 (drop n1 l).
-  Proof using.
-    intros. rewrite !drop_drop. f_equal. lia.
-  Qed.  
-
-  Lemma dequeue_restore_QI 
-  (h : nat)
-  (ph : loc)
-  (vh : val)
-  (nxh : loc)
-  (fl : nat)
-  (hq : HistQueue)
-  (t br : nat)
-  (HTH : hq !! h = Some (ph, (vh, nxh)))
-  (T_LEN : t = length hq)
-  (pt : loc)
-  (LL : is_LL_into (drop h hq) pt):
-  ⊢ ([∗ list] nd ∈ drop h hq, hn_interp nd) -∗
-  Tail q_sq ↦{1 / 2} #pt -∗ 
-  tail_interp pt -∗
-  Head q_sq ↦{1 / 2} #nxh -∗
-  (∃ nbr : HistNode, ⌜hq !! br = Some nbr⌝ ∗ BeingRead q_sq ↦ #nbr.1) -∗ 
-  (∃ nfl : HistNode, ⌜hq !! fl = Some nfl⌝ ∗ FreeLater q_sq ↦ #nfl.1 ∗
-    hn_interp nfl) -∗ 
-  queue_interp hq (h + 1) t br fl ∗ hn_interp (ph, (vh, nxh)).
-  Proof using. 
-    iIntros "Q TAIL DUMMY HEAD BL FL".
-    rewrite /queue_interp. 
-    iFrame.
-    rewrite -!bi.sep_assoc.
-    iSplit; [done| ].
-    iFrame "%".
-    pose proof (take_drop_middle _ _ _ HTH) as SPLIT.
-    rewrite -SPLIT.
-    assert (length (take h hq) = h) as H_LEN. 
-    { apply length_take_le. apply lookup_lt_Some in HTH.
-      (* simpl in *. lia. *)
-      apply Nat.le_lteq. tauto. }
-    rewrite drop_app_length'; [| done]. simpl.
-    rewrite cons_middle app_assoc.
-    rewrite drop_app_length'.
-    2: { rewrite length_app /=.
-         (* clear -H_LEN. lia. *)
-         by rewrite H_LEN. }
-    iDestruct "Q" as "[$ $]".
-    iSplit.
-    { iPureIntro. rewrite -(drop_drop _ _ 1) drop_drop_comm.  
-      apply is_LL_into_drop; auto. } 
-    rewrite -SPLIT in LL.
-    rewrite drop_app_length' in LL; [| done].
-    simpl in LL. destruct (drop (S h) hq) eqn:REST.
-    all: rewrite REST in LL; rewrite REST /=.
-    - subst. simpl. iFrame.
-    - simpl. destruct h0 as [? [??]]. simpl.
-      destruct LL as [-> ?]. by iFrame.
-  Qed.
-
-  Lemma dequeue_upd_head_post (τ : locale heap_lang) (π : Phase) (q : Qp)
-    (h : nat) (ph : loc) (vh : val) (nxh : loc) (fl : nat)
-    (hq : HistQueue) (t br : nat) (rop : option nat) (hist : read_hist)
-  (ORDER : hq_state_wf h t br fl)
-  (HTH : hq !! h = Some (ph, (vh, nxh)))
-  (NEMPTY : t ≠ h)
-  (T_LEN : t = length hq)
-  (pt : loc)
-  (LL : is_LL_into (drop h hq) pt):
-  ith_node h (ph, (vh, nxh)) -∗ 
-  @me_exact _ q_me_h h -∗
-  @me_exact _ q_me_fl fl -∗
-  dangle_frag None -∗
-  hq_auth hq -∗
-  auths h t br fl -∗
-  ([∗ list] nd ∈ drop h hq, hn_interp nd) -∗
-  Tail q_sq ↦{1 / 2} #pt -∗
-  tail_interp pt -∗
-  (∃ nbr : HistNode, ⌜hq !! br = Some nbr⌝ ∗ BeingRead q_sq ↦ #nbr.1) -∗
-  (∃ nfl : HistNode, ⌜hq !! fl = Some nfl⌝ ∗ FreeLater q_sq ↦ #nfl.1 ∗
-           hn_interp nfl) -∗
-  dangle_auth None -∗
-  ohv_interp -∗
-  read_hist_interp hist rop h br fl None -∗
-  ((∃ pt0 : loc, read_head_resources t br pt0 None ∗ rop_token)
-         ∨ read_head_token) -∗
-  dequeue_token -∗
-  (▷ (∃ (hq0 : HistQueue) (h0 t0 br0 fl0 : nat) 
-                (rop0 od : option nat) (hist0 : read_hist),
-                queue_inv_inner hq0 h0 t0 br0 fl0 rop0 od hist0) ={
-           ⊤ ∖ ↑queue_ns,⊤}=∗ emp) -∗
-  Head q_sq ↦{1 / 2} #nxh -∗
-  Head q_sq ↦{1 / 2} #nxh -∗
-  |={⊤ ∖ ↑queue_ns,⊤}=> 
-    (@me_exact _ q_me_h (h + 1) ∗ @me_exact _ q_me_fl fl ∗ Head q_sq ↦{1 / 2} #nxh ∗
-     dangle_frag (Some h)) ∗
-    ∃ i r b : nat, ith_read i r (h + 1) ∗ ⌜r ≤ h⌝ ∗ br_lb b ∗
-      (⌜b < r⌝ -∗
-       ith_rp i rs_canceled
-       ∨ ith_rp i rs_aborted ∨ ith_rp i (rs_proc (Some rsp_completed))).
-  Proof using. 
-    iIntros "#HTH CH CFL DFRAG HQ AUTHS Q TAIL DUMMY BR FL DAUTH OHV RHI RH TOK CLOS HEAD HEAD'".
-
-    iMod (dangle_update _ _ (Some h) with "[$] [$]") as "[DAUTH DFRAG]".
-
-    iAssert (|==> auths (h + 1) t br fl ∗ @me_exact _ q_me_h (h + 1))%I with "[CH AUTHS]" as "UPD".
-    { rewrite /auths. iDestruct "AUTHS" as "(AUTH&?&?&?)". iFrame.
-      iApply (me_update with "AUTH CH"). lia. }
-    iMod "UPD" as "[AUTHS CH]".
-
-    iFrame.
-
-    iDestruct (dequeue_restore_QI with "[$] [$] [$] [$] [$] [$]") as "[QI HNI]".
-    all: try by eauto. 
-
-    iDestruct (cancel_rop with "[$]") as "#CNC".
-    { red. rewrite Nat.add_1_r. reflexivity. }
-    
-    iDestruct (take_snapshot with "[$]") as "#SHT".
-    iDestruct "SHT" as "(_&_&#BR_LB&_)". 
-
-    rewrite /read_hist_interp. iDestruct "RHI" as "(ROPA & ROP & RHIST & %RH_WF & #OLDS)". 
-    rewrite /rop_interp.
-    destruct rop as [n| ]. 
-    - iDestruct ("ROP" with "[//]") as "(%r & %rp & READ_ & RP & ROP)".      
-      destruct RH_WF as (n' & DOM & [? | [=]] & RH_WF); [done| ]. subst n'. 
-      iMod (read_hist_wf_bump with "[$] [RP]") as "(%r' & %rp' & RHIST & #READ & %RH_WF' & RP & %READ_BOUND)".
-      { eexists. eauto. }
-      { rewrite DOM dom_max_set_fold. iFrame. }
-      rewrite DOM dom_max_set_fold. 
-      iDestruct (ith_read_agree with "READ READ_") as %<-.
-      iFrame "READ". iFrame "%". iFrame "BR_LB". 
-      rewrite -(bi.sep_True' ( ⌜ _ ⌝ -∗ _ )%I). iApply fupd_frame_l. iSplit.
-      { iIntros (LT). iDestruct "ROP" as "[SAFE | [-> _]]".
-        2: { iFrame. }
-        iDestruct "SAFE" as "[FROM_HEAD | [FROM_DANGLE | FROM_BR]]".
-        - iDestruct "FROM_HEAD" as "[-> [-> | (-> & -> & ?)]]".
-          + simpl. iFrame. 
-          + lia. 
-        - iDestruct "FROM_DANGLE" as "[(-> & -> & %X) ?]".
-          clear -X. by destruct X. 
-        - iDestruct "FROM_BR" as "([-> ->] & -> & ?)". lia. } 
-
-      iClear "HTH".
-      iMod ("CLOS" with "[-]") as "_"; [| done].
-      iFrame "QI AUTHS OHV HQ RH DAUTH TOK RHIST ROPA". iNext.
-      rewrite Nat.add_sub. rewrite HTH /=. 
-      
-      iSplit.
-      { iPureIntro. red. red in ORDER. repeat split; try lia. }
-      iSplitL "HNI". 
-      { iRight. by iFrame. }
-      rewrite DOM dom_max_set_fold in RH_WF'.
-      iFrame "%". 
-      iSplit.
-      2: { iApply old_rps_olds.
-           iDestruct (old_rps_olds with "OLDS") as "foo". 
-           by rewrite delete_insert_delete. }
-      rewrite /rop_interp. iIntros (i_ [=]). subst i_. 
-
-      iFrame "READ_ RP". 
-      iDestruct "ROP" as "[[HEAD | [DANGLE | FL]] | CANCEL_WITNESS]".
-      + iDestruct "HEAD" as "(-> & [-> | (-> & -> & ?)])".
-        * iRight. simpl. by iFrame "#∗".
-        * iLeft. iRight. iLeft. iFrame.
-          iPureIntro. split.
-          ** split; [lia | done].
-          ** simpl. done. 
-      + iDestruct "DANGLE" as "((_ & _ & %) & _)". by destruct H.
-      + iDestruct "FL"as "([-> ->] & -> & ?)". 
-        iLeft. rewrite /safe_read. iFrame. 
-        repeat iRight. iFrame. done.
-      + iDestruct "CANCEL_WITNESS" as "(-> & CW)".
-        iRight. by iFrame.
-    - destruct RH_WF as (n & DOM & [? | [=]] & RH_WF).
-      destruct (hist !! n) as [[[??]?] | ] eqn:NTH. 
-      2: { apply not_elem_of_dom in NTH. rewrite DOM in NTH.
-           rewrite elem_of_set_seq in NTH. lia. }
-      iDestruct (big_sepM_lookup with "OLDS") as "RP".
-      { simpl. apply NTH. } 
-      iDestruct "RP" as "(%rp & RP & %FIN & #LB)".
-      iDestruct (ith_rp_hist_compat with "[$] [$]") as %(? & ? & LE').
-      rewrite NTH in H0. inversion H0. subst x. simpl in *.
-
-      iDestruct (read_hist_get hist n with "RHIST") as "#READ".
-      { rewrite NTH. repeat f_equal. }
-      
-      iMod (read_hist_wf_bump with "[$] [RP]") as "(%r' & %rp' & RHIST & #READ' & %RH_WF' & RP_ & %READ_BOUND)".
-      { eexists. eauto. }
-      { rewrite DOM dom_max_set_fold. iFrame "RP". }
-      rewrite DOM dom_max_set_fold.
-      iDestruct (ith_read_agree with "READ READ'") as %->.
-      iFrame "% READ' BR_LB".
-      rewrite -(bi.sep_True' ( ⌜ _ ⌝ -∗ _ )%I). iApply fupd_frame_l. iSplit.
-      { iIntros (LT). destruct FIN as [-> | [-> | [-> | ->]]].
-        all: try by iFrame.
-        iDestruct "LB" as "[LB | [%RS_AB | %RS_CANC]]".
-        2, 3: done. 
-        iDestruct (br_lb_bound with "[$] [$]") as %?. lia. }
-
-      iMod ("CLOS" with "[-]") as "_"; [| done].
-      iFrame "QI AUTHS OHV HQ RH DAUTH TOK RHIST". iNext.
-      iExists _. rewrite Nat.add_sub. rewrite HTH /=.
-      
-      iSplit.
-      { iPureIntro. red. red in ORDER. repeat split; try lia. }
-      iSplitL "HNI". 
-      { iRight. by iFrame. }
-      rewrite DOM dom_max_set_fold in RH_WF'.
-      destruct RH_WF as (SEQ &  BB). 
-      Unshelve. 2: exact None. 
-      rewrite bi.sep_assoc.
-      iFrame "ROPA". 
-      rewrite /rop_interp. iSplit. 
-      { iIntros (i_ [=]). }
-      iSplitR.
-      2: { (* TODO: make a lemma? *)
-        rewrite /old_rps. simpl.
-        rewrite -insert_delete_insert.         
-        rewrite insert_union_singleton_l big_sepM_union.
-        2: { apply map_disjoint_dom. rewrite dom_insert_L. set_solver. }
-        iSplitL.
-        2: { iApply (big_sepM_subseteq with "[$]"). apply delete_subseteq. }
-        rewrite big_sepM_singleton. iFrame. iFrame "% #".
-        iSplit. 
-        { iPureIntro. by apply upd_rp_fin_pres. }
-        iDestruct "LB" as "[$ | [-> | ->]]".
-        all: simpl; iRight; iPureIntro; tauto. }
-
-      (* TODO: make a lemma *)
-      rewrite /read_hist_wf.
-      iPureIntro. 
-
-      exists n. split; [| split; [| split]]. 
-    + rewrite dom_insert_L. apply mk_is_Some, elem_of_dom in NTH. set_solver.
-    + tauto. 
-    + intros ?????. rewrite !lookup_insert_Some.
-      intros [(? & ?) | (? & ITH) ] [(? & ?) | (? & JTH) ]; subst; simpl in *; try lia.
-      * apply mk_is_Some, elem_of_dom in JTH.
-        rewrite DOM elem_of_union elem_of_set_seq elem_of_singleton in JTH. lia.
-      * eapply SEQ in H1; eauto. done.
-      * eapply SEQ; eauto.
-    + intros ??. rewrite lookup_insert_Some.         
-      intros [(? & ?) | (? & ITH) ]; subst; simpl; try lia.
-      eapply BB in ITH; eauto. simpl in ITH. lia.
-  Qed.
-
-End DequeueGhost.
 
 
 Definition free_el: val :=
@@ -509,7 +160,7 @@ Section Dequeue.
   Qed.
 
   Definition dequeue_fuel := 100.    
-
+  
   Lemma check_BR_spec l τ π q h fl ph ndh i r b0
     (READ_BOUND: r <= h):
     {{{ queue_inv l ∗
@@ -554,79 +205,7 @@ Section Dequeue.
     MU_by_burn_cp. iApply wp_value.
 
     iApply "POST". iFrame.
-
-    iDestruct (br_lb_bound with "BR0 AUTHS") as %BR0. 
-    iDestruct (take_snapshot with "[$]") as "#SHT".
-    iDestruct (hq_auth_get_ith with "HQ") as "#BRTH'".
-    { apply BRTH. }
-    iFrame "BRTH'". 
-
-    iAssert (queue_interp hq (h + 1) t br fl)%I with "[PQI BR FL]" as "QI".
-    { by iFrame. }
-    iAssert (br_lb br ∗ ⌜b0 ≤ br⌝)%I as "$".
-    { iSplit; [| done].
-      iDestruct "SHT" as "(?&?&?&?)". done. }
-
-    simpl.
-    destruct (decide (pbr = ph)) as [-> | NEQ].
-    -
-      iFrame. 
-      iMod ("CLOS" with "[-]") as "_".
-      { iFrame "#∗ %". iNext.
-        rewrite Nat.add_sub HTH /=.
-        iRight. by iFrame. }
-      iModIntro. by iLeft.
-    - rewrite /read_hist_interp. iDestruct "RHI" as "(ROPA & ROP & RHIST & %RH_WF & #OLDS)".  
-      iDestruct (ith_read_hist_compat with "[$] [$]") as %(b & p & READ & INCR_BOUND). 
-      iMod (dangle_update _ _ None with "[$] [$]") as "[DAUTH DFRAG]".
-      iFrame.      
-      iApply fupd_or. iRight. iFrame "HNI".
-      rewrite -(bi.sep_True' ⌜ _ ≠ _ ⌝%I). iApply fupd_frame_l. iSplit; [done| ].
-      iMod ("CLOS" with "[-]") as "_"; [| done]. 
-
-      rewrite /rop_interp.
-      destruct rop.
-      2: { iFrame "#∗ %". iNext. iSplitR.
-           { by iLeft. }
-           rewrite /rop_interp. by iIntros (??). }
-      
-      iDestruct ("ROP" with "[//]") as "(%r_ & %rp & READ_ & RP & ROP)".
-      iDestruct (ith_read_hist_compat with "[$] READ_") as %(?&? & READ' & _). 
-
-      iFrame. iFrame "OLDS".
-      iNext. iFrame (RH_WF ORDER). iSplitR.
-      { by iLeft. }
-      rewrite /rop_interp.
-      iIntros (i' [=]). subst n.
-      iDestruct "ROP" as "[SAFE | $]".
-      2: { iFrame "#∗". }
-
-      destruct (decide (i' = i)). 
-      { subst. rewrite {1}/safe_read. rewrite Nat.add_sub.
-        iFrame "READ_". 
-        iDestruct "SAFE" as "[FROM_HEAD | [FROM_DANGLE | FROM_BR]]".
-        - iFrame.
-        - iDestruct "FROM_DANGLE" as "[(-> & -> & _) ?]".
-          congruence.
-        - iFrame. }
-
-      assert (i < i') as NEW.
-      { red in RH_WF. destruct RH_WF as (n' & DOM & [? | [=]] & RH_WF); [done| ].
-        subst i'.
-        apply mk_is_Some, elem_of_dom in READ. rewrite DOM elem_of_set_seq in READ.
-        lia. }
-      clear n.
-      
-      assert (h + 1 <= r_) as READ'_BOUND.
-      { red in RH_WF. destruct RH_WF as (n' & DOM & [? | [=]] & RH_WF); [done| ].
-        subst. 
-        apply proj1 in RH_WF. eapply RH_WF in NEW; eauto. simpl in NEW. lia. }
-      iFrame "READ_".
-      rewrite {1}/safe_read.
-      iDestruct "SAFE" as "[FROM_HEAD | [FROM_DANGLE | FROM_BR]]".
-      + iFrame.
-      + iDestruct "FROM_DANGLE" as "[(-> & -> & _) ?]". lia.
-      + iFrame.
+    iApply (check_BR_post with "[$] [$] [$] [$] [$] [$] [$] [$] [$] [$] [$] [$] [$] [$] [$]"); eauto.
   Qed.
 
   Lemma read_FL_spec τ π l h q fl nd od:
@@ -723,133 +302,40 @@ Section Dequeue.
 
     iClear "INV QAT".
 
+    iPoseProof (queue_interp_dangle_neq_pfl' _ _ _ _ _ ph with "QI [DANGLE]") as "#PFL_NEQ_D".
+    { by rewrite Nat.add_sub. }
+
+    rewrite /dangle_interp. iDestruct "DANGLE" as "(DAUTH & [% | (_ & HNI)])"; [done| ].
+
     (* TODO: split into lemmas *)
     iDestruct (hq_auth_lookup with "[$] HTH") as %HTH.
     iAssert (⌜ t ≠ h ⌝)%I as %NEMPTY.
     { iIntros (->). red in ORDER. lia. }
 
-    iPoseProof (queue_interp_dangle_neq_pfl' _ _ _ _ _ ph with "QI [DANGLE]") as "#PFL_NEQ_D".
-    { by rewrite Nat.add_sub. }
-
-    rewrite /dangle_interp. iDestruct "DANGLE" as "(DAUTH & [% | (_ & HNI)])"; [done| ].
     rewrite Nat.add_sub HTH /=. 
     rewrite /dequeue_resources. iDestruct "DR" as "(CH & CFL & HEAD' & DFRAG)".
-
     
     rewrite /queue_interp. iDestruct "QI" as "(%T_LEN & PQI & BR & FL)".
-    iDestruct "BR" as "(%nbr & %BRTH & BR)".    
-    iDestruct (br_lb_bound with "BR1 AUTHS") as %BR1. 
-
-    subst pbr. 
-    destruct nbr as [pbr nbr].
-
-    (* iCombine "HEAD HEAD'" as "HEAD".  *)
-    iApply sswp_MU_wp; [done| ].
 
     iDestruct "FL" as "(%ndfl_ & %FLTH & FL & HNI_FL)".
     iDestruct (hq_auth_lookup with "[$] FLTH") as %FLTH_.
     rewrite FLTH in FLTH_. inversion FLTH_. subst ndfl_. clear FLTH_. 
+
+    iApply sswp_MU_wp; [done| ].
     iApply (wp_store with "FL"). iIntros "!> FL".
     MU_by_burn_cp. iApply wp_value.
 
-    iMod (dangle_update _ _ None with "[$] [$]") as "[DAUTH DFRAG]".
-    iAssert (|==> auths (h + 1) t br h ∗ @me_exact _ q_me_fl h)%I with "[CFL AUTHS]" as "UPD".
-    { rewrite /auths. iDestruct "AUTHS" as "(?&?&?&A)". iFrame.
-      iApply (me_update with "A CFL"). red in ORDER. lia. }
-    iMod "UPD" as "[AUTHS CFL]".
+    iAssert (|={⊤ ∖ ↑queue_ns,⊤}=> ∃ (hn : Node) (fl' : nat),
+    (let '(v, nxt) := hn in pfl ↦ v ∗ (pfl +ₗ 1) ↦ #nxt) ∗ 
+    th_phase_frag τ π q ∗ @me_exact _ q_me_h (h + 1) ∗ me_exact fl' ∗
+    simple_queue.Head q_sq ↦{1 / 2} #ndh.2 ∗ dangle_frag None)%I with "[-POST CPS]" as "UPD".
+    2: { iMod "UPD" as "(%&%&?&PH&?&?&?&?)". iModIntro.
+         wp_bind (Rec _ _ _)%E. pure_steps.
+         iApply "POST". iFrame. }
 
-    iDestruct (br_lb_bound with "BR0 [$]") as %BR0. 
-    iAssert (queue_interp hq (h + 1) t br h)%I
-      with "[PQI BR FL HNI]" as "QI".
-    { iFrame. iSplit; [done| ].
-      iFrame "%". iFrame. }
+    iFrame "PH".
 
-    rewrite /read_hist_interp. iDestruct "RHI" as "(ROPA & ROP & RHIST & %RH_WF & #OLDS)". 
-    rewrite /rop_interp.
-    destruct rop. 
-    - iDestruct ("ROP" with "[//]") as "(%r_ & %rp & READ_ & RP & ROP)".
-      iDestruct (ith_read_hist_compat with "[$] READ_") as %(?&? & READ' & _). 
-      iDestruct (ith_read_hist_compat with "[$] READ") as %(?&? & READ & BB).
-      iDestruct (hq_auth_lookup with "[$] BRTH1") as %BRTH1.
-      
-      iAssert (dequeue_resources (h + 1) h ndh.2 None)%I with "[CH CFL HEAD' DFRAG]" as "DR".
-      { iFrame. }
-
-      iMod ("CLOS" with "[-POST CPS PH DR HNI_FL]") as "_".
-      { iFrame. iNext. iFrame "OLDS". iFrame (RH_WF).
-        iSplit. 
-        { rewrite /hq_state_wf. iPureIntro. red in ORDER. lia. }
-        iSplitR.
-        { by iLeft. }        
-        rewrite /rop_interp.
-        iIntros (i' [=]). subst n.
-        iDestruct "ROP" as "[SAFE | $]".
-        2: { iFrame. }
-        iFrame "READ_".
-          
-        destruct (decide (i' = i)). 
-        { subst. rewrite {1}/safe_read. rewrite Nat.add_sub.
-          iDestruct "SAFE" as "[FROM_HEAD | [FROM_DANGLE | FROM_BR]]".
-          - iFrame.
-          - iDestruct "FROM_DANGLE" as "((-> & -> & _) & -> & ?)".
-            iFrame "RP". 
-            iLeft. rewrite /safe_read. rewrite Nat.add_sub.
-            do 2 iRight. by iFrame. 
-          - iDestruct "FROM_BR" as "([-> ->] & -> & ?)". 
-            rewrite READ in READ'. inversion READ'. subst r x1 x2.
-            apply Nat.le_lteq in BR0 as [BR0 | ->].
-            { iSpecialize ("NO_FL" with "[//]"). iExFalso.
-              iAssert (∃ rp', ith_rp i rp' ∗ ⌜ rp' = rs_canceled \/ rp' = rs_aborted \/ rp' = (rs_proc (Some rsp_completed))⌝)%I as "(%rp' & RP' & %RP')".
-              { iDestruct "NO_FL" as "[$|[$|$]]"; set_solver. }
-              iDestruct (ith_rp_le with "RP RP'") as %CM.
-              exfalso. clear -RP' CM.
-              inversion CM; destruct RP' as [-> | [-> | ->]]; try done.
-              subst. inversion RSP. by subst. }
-            rename x into bi.
-            red in RH_WF.
-            destruct RH_WF as (n' & DOM & [? | [=]] & SEQ & BB'); [done| ].
-            subst n'.
-            pose proof READ as EQ%BB'. simpl in EQ.
-            assert (bi = h + 1) as -> by lia.  clear BB EQ.
-            assert (b1 = fl) as -> by lia.
-            rewrite BRTH in BRTH1. inversion BRTH1. subst pbr ndbr1.
-            iDestruct ("PFL_NEQ_D" with "[] []") as "?".
-            { eauto. }
-            { eauto. }
-            done. }
-          
-        assert (i < i') as NEW.
-        { red in RH_WF. destruct RH_WF as (n' & DOM & [? | [=]] & RH_WF); [done| ].
-          subst i'.
-          apply mk_is_Some, elem_of_dom in READ. rewrite DOM elem_of_set_seq in READ.
-          lia. }
-        clear n.
-
-        assert (h + 1 <= r_) as READ'_BOUND.
-        { red in RH_WF. destruct RH_WF as (n' & DOM & [? | [=]] & RH_WF); [done| ].
-          apply proj1 in RH_WF. eapply RH_WF in NEW; eauto. simpl in NEW. lia. }
-        rewrite {1}/safe_read.
-        iDestruct "SAFE" as "[FROM_HEAD | [FROM_DANGLE | FROM_BR]]".
-        + iFrame.
-        + iDestruct "FROM_DANGLE" as "[(-> & -> & _) ?]". lia.
-        + iFrame.
-          iDestruct "FROM_BR" as "([% %] & ?)". subst.
-          red in ORDER. lia. }
-      iModIntro. wp_bind (Rec _ _ _)%E. pure_steps.
-      iApply "POST". iFrame. 
-    - 
-      iAssert (dequeue_resources (h + 1) h ndh.2 None)%I with "[CH CFL HEAD' DFRAG]" as "DR".
-      { iFrame. }
-
-      iMod ("CLOS" with "[-POST CPS PH DR HNI_FL]") as "_".
-      { iFrame. iNext. iFrame "OLDS". iFrame (RH_WF). iSplit.
-        { rewrite /hq_state_wf. iPureIntro. red in ORDER. lia. }
-        iSplitR.
-        { by iLeft. }
-        rewrite /rop_interp. by iIntros (??). }
-
-      iModIntro. wp_bind (Rec _ _ _)%E. pure_steps.
-      iApply "POST". iFrame. 
+    iApply (get_to_free_post with "HTH READ BR0 NO_FL BR1 BRTH1 FLTH PFL_NEQ_D [$] [$] [$] [$] [$] [$] [$] [$] [$] [$] [$] [$] [$] [$] [$] [$] [$]"); eauto. 
   Qed.
 
   Lemma free_el_spec τ π q ptr nd:
@@ -863,12 +349,6 @@ Section Dequeue.
     rewrite /free_el.
     pure_steps.
 
-    (* iApply sswp_MU_wp; [done| ]. *)
-    (* iApply sswp_pure_step; [done| ]. *)
-    (* MU_by_burn_cp. rewrite loc_add_0. iApply wp_value. *)
-    
-    (* wp_bind (Free _)%E. *)
-    (* replace Free with (AllocN #1) by admit.   *)
     wp_bind (_ +ₗ _)%E.
     iApply sswp_MU_wp; [done| ].
     iApply sswp_pure_step; [done| ].
@@ -924,7 +404,6 @@ Section Dequeue.
     { by iFrame. }
     iModIntro.
 
-    (* TODO: do we need to keep track of previous values at this point? *)
     clear t br ORDER hq.
     clear pt rop hist.
 
@@ -961,7 +440,6 @@ Section Dequeue.
     { set_solver. }
     MU_by_burn_cp. iApply wp_value.
 
-    (* destruct bool_decide. *)
     iDestruct "HT" as "[[%GE <-] | (%NEMPTY & %ndh & #HTH)]". 
     { assert (t = h) as ->.
       { red in ORDER. lia. }
@@ -1034,7 +512,6 @@ Section Dequeue.
     iDestruct "inv" as ">(HQ & AUTHS & %ORDER & QI & DANGLE & OHV & RHI & RH & DQ)".
     iDestruct "DQ" as "[(% & DR') | TOK]".
     { by iDestruct (dequeue_resources_excl with "DR DR'") as "?". }
-    (* iDestruct (dequeue_res_head_agree with "DR [$]") as %->.  *)
     iDestruct (dequeue_resources_auth_agree with "DR [$]") as %[<- <-].
     iDestruct (dequeue_resources_dangle_agree with "DR [$]") as %->.
 
