lawyer/nonblocking/examples/queue/dequeuer/dequeue_ghost.v
@@ -1,0 +1,635 @@
+From iris.base_logic Require Export gen_heap.
+From iris.proofmode Require Import tactics coq_tactics.
+From iris.bi.lib Require Import fixpoint.
+From fairness Require Import utils.
+From iris.algebra Require Import auth gmap gset excl excl_auth csum mono_nat.
+From iris.base_logic.lib Require Import invariants.
+From lawyer.nonblocking.examples.queue Require Import simple_queue_utils simple_queue.
+(* From lawyer.nonblocking.examples.queue.dequeuer Require Import (* dequeuer_lib *). *)
+From heap_lang Require Import heap_lang_defs lang notation.
+
+Close Scope Z.
+
+
+Section DequeueGhost.
+  Context {Σ} {hG: heap1GS Σ} {iG: invGS_gen HasNoLc Σ}.  
+  Context {QL: QueueG Σ}.
+  
+  (* TODO: move *)
+  Lemma is_LL_into_drop hq pt k
+    (LL: is_LL_into hq pt):
+    is_LL_into (drop k hq) pt.
+  Proof using.
+    revert k. induction hq.
+    { intros. by rewrite drop_nil. }
+    intros. destruct k.
+    { by rewrite drop_0. }
+    simpl. apply IHhq.
+    simpl in LL. destruct a as [? [? ?]].
+    destruct hq; try done.
+    destruct h as [? [? ?]]. tauto.
+  Qed.
+
+  (* TODO: move *)
+  Lemma dom_max_set_fold n:
+    set_fold max 0 (set_seq 0 (S n): gset nat) = n.
+  Proof using.
+    clear. induction n.
+    { done. }
+    rewrite set_seq_S_end_union_L.
+    rewrite union_comm_L. 
+    erewrite set_fold_union.
+    2-4: red; lia.
+    simpl. rewrite IHn.
+    rewrite set_fold_singleton. lia.
+  Qed.
+
+  Definition upd_rp rp :=
+    match rp with
+    | rs_init => rs_canceled
+    | rs_proc (Some rsp_going) => rs_proc (Some rsp_protected)
+    | _ => rp
+    end. 
+
+  Lemma upd_rp_rs_step p: rs_step p (upd_rp p).
+  Proof using.
+    destruct p; simpl; try constructor.
+    destruct orsp; simpl; try constructor.
+    destruct r; repeat constructor.
+  Qed.
+
+  Lemma read_hist_wf_bump (hist: read_hist) rop h rp
+    (RH_WF: read_hist_wf hist rop h)
+    (n := set_fold max 0 (dom hist)):
+    read_hist_auth hist -∗ ith_rp n rp ==∗
+    ∃ r rp', let hist' := <[ n := ((r, h + 1), rp') ]> hist in
+      read_hist_auth hist' ∗ ith_read n r (h + 1) ∗ ⌜ read_hist_wf hist' rop (h + 1) ⌝ ∗
+      ith_rp n (upd_rp rp) ∗ ⌜ r <= h ⌝.
+  Proof using.
+    rewrite /read_hist_wf. iIntros "AUTH RP".
+    destruct RH_WF as (n_ & DOM & ROP & SEQ & BB).
+
+    assert (n_ = n) as ->.
+    { subst n. rewrite DOM. by rewrite dom_max_set_fold. }
+
+    destruct (hist !! n) as [[[r b0] p]| ] eqn:NTH.
+    2: { apply not_elem_of_dom in NTH. rewrite DOM in NTH.
+         rewrite elem_of_set_seq in NTH. lia. }
+    iDestruct (ith_rp_hist_compat with "[$] [$]") as %(? & ? & EQ').
+    rewrite NTH in H. inversion H. subst x. simpl in EQ'. clear H.
+    rename rp into p_. 
+    
+    iMod (read_hist_update' _ _ _ _ _ (h + 1) with "AUTH RP") as "(AUTH & #ITH & RP)".
+    { apply upd_rp_rs_step. }
+    { apply NTH. }
+
+    rewrite Nat.max_r.
+    2: { apply BB in NTH. simpl in NTH. lia. }
+    iModIntro. do 2 iExists _. iFrame "AUTH ITH RP".
+    iPureIntro. split.
+    2: { eapply BB in NTH; eauto. by apply NTH. }
+
+    exists n. split; [| split; [| split]]. 
+    - rewrite dom_insert_L. apply mk_is_Some, elem_of_dom in NTH. set_solver.
+    - done.
+    - intros ?????. rewrite !lookup_insert_Some.
+      intros [(? & ?) | (? & ITH) ] [(? & ?) | (? & JTH) ]; subst; simpl in *; try lia.
+      + apply mk_is_Some, elem_of_dom in JTH.
+        rewrite DOM elem_of_union elem_of_set_seq elem_of_singleton in JTH. lia.
+      + eapply SEQ in H; eauto. done.
+      + eapply SEQ; eauto.
+    - intros ??. rewrite lookup_insert_Some.         
+      intros [(? & ?) | (? & ITH) ]; subst; simpl; try lia.
+      { eapply BB in NTH; eauto. simpl in NTH. lia. }
+      eapply BB in ITH; eauto. lia.
+  Qed.
+
+  Lemma upd_rp_fin_pres rs
+    (FIN: rs_fin rs):
+    rs_fin (upd_rp rs).
+  Proof using.
+    red. destruct FIN as [-> | [-> | [-> | ->]]]; subst; simpl; try by eauto.
+  Qed.
+
+  (* TODO: move *)
+  Lemma drop_drop_comm: ∀ {A : Type} (l : list A) (n1 n2 : nat),
+      drop n1 (drop n2 l) = drop n2 (drop n1 l).
+  Proof using.
+    intros. rewrite !drop_drop. f_equal. lia.
+  Qed.  
+
+  Lemma dequeue_restore_QI 
+  (h : nat)
+  (ph : loc)
+  (vh : val)
+  (nxh : loc)
+  (fl : nat)
+  (hq : HistQueue)
+  (t br : nat)
+  (HTH : hq !! h = Some (ph, (vh, nxh)))
+  (T_LEN : t = length hq)
+  (pt : loc)
+  (LL : is_LL_into (drop h hq) pt):
+  ⊢ ([∗ list] nd ∈ drop h hq, hn_interp nd) -∗
+  Tail q_sq ↦{1 / 2} #pt -∗ 
+  tail_interp pt -∗
+  Head q_sq ↦{1 / 2} #nxh -∗
+  (∃ nbr : HistNode, ⌜hq !! br = Some nbr⌝ ∗ BeingRead q_sq ↦ #nbr.1) -∗ 
+  (∃ nfl : HistNode, ⌜hq !! fl = Some nfl⌝ ∗ FreeLater q_sq ↦ #nfl.1 ∗
+    hn_interp nfl) -∗ 
+  queue_interp hq (h + 1) t br fl ∗ hn_interp (ph, (vh, nxh)).
+  Proof using. 
+    iIntros "Q TAIL DUMMY HEAD BL FL".
+    rewrite /queue_interp. 
+    iFrame.
+    rewrite -!bi.sep_assoc.
+    iSplit; [done| ].
+    iFrame "%".
+    pose proof (take_drop_middle _ _ _ HTH) as SPLIT.
+    rewrite -SPLIT.
+    assert (length (take h hq) = h) as H_LEN. 
+    { apply length_take_le. apply lookup_lt_Some in HTH.
+      (* simpl in *. lia. *)
+      apply Nat.le_lteq. tauto. }
+    rewrite drop_app_length'; [| done]. simpl.
+    rewrite cons_middle app_assoc.
+    rewrite drop_app_length'.
+    2: { rewrite length_app /=.
+         (* clear -H_LEN. lia. *)
+         by rewrite H_LEN. }
+    iDestruct "Q" as "[$ $]".
+    iSplit.
+    { iPureIntro. rewrite -(drop_drop _ _ 1) drop_drop_comm.  
+      apply is_LL_into_drop; auto. } 
+    rewrite -SPLIT in LL.
+    rewrite drop_app_length' in LL; [| done].
+    simpl in LL. destruct (drop (S h) hq) eqn:REST.
+    all: rewrite REST in LL; rewrite REST /=.
+    - subst. simpl. iFrame.
+    - simpl. destruct h0 as [? [??]]. simpl.
+      destruct LL as [-> ?]. by iFrame.
+  Qed.
+
+  Lemma dequeue_upd_head_post (τ : locale heap_lang)
+    (h : nat) (ph : loc) (vh : val) (nxh : loc) (fl : nat)
+    (hq : HistQueue) (t br : nat) (rop : option nat) (hist : read_hist)
+  (ORDER : hq_state_wf h t br fl)
+  (HTH : hq !! h = Some (ph, (vh, nxh)))
+  (NEMPTY : t ≠ h)
+  (T_LEN : t = length hq)
+  (pt : loc)
+  (LL : is_LL_into (drop h hq) pt):
+  ith_node h (ph, (vh, nxh)) -∗ 
+  @me_exact _ q_me_h h -∗
+  @me_exact _ q_me_fl fl -∗
+  dangle_frag None -∗
+  hq_auth hq -∗
+  auths h t br fl -∗
+  ([∗ list] nd ∈ drop h hq, hn_interp nd) -∗
+  Tail q_sq ↦{1 / 2} #pt -∗
+  tail_interp pt -∗
+  (∃ nbr : HistNode, ⌜hq !! br = Some nbr⌝ ∗ BeingRead q_sq ↦ #nbr.1) -∗
+  (∃ nfl : HistNode, ⌜hq !! fl = Some nfl⌝ ∗ FreeLater q_sq ↦ #nfl.1 ∗
+           hn_interp nfl) -∗
+  dangle_auth None -∗
+  ohv_interp -∗
+  read_hist_interp hist rop h br fl None -∗
+  ((∃ pt0 : loc, read_head_resources t br pt0 None ∗ rop_token)
+         ∨ read_head_token) -∗
+  dequeue_token -∗
+  (▷ (∃ (hq0 : HistQueue) (h0 t0 br0 fl0 : nat) 
+                (rop0 od : option nat) (hist0 : read_hist),
+                queue_inv_inner hq0 h0 t0 br0 fl0 rop0 od hist0) ={
+           ⊤ ∖ ↑queue_ns,⊤}=∗ emp) -∗
+  Head q_sq ↦{1 / 2} #nxh -∗
+  Head q_sq ↦{1 / 2} #nxh -∗
+  |={⊤ ∖ ↑queue_ns,⊤}=> 
+    (@me_exact _ q_me_h (h + 1) ∗ @me_exact _ q_me_fl fl ∗ Head q_sq ↦{1 / 2} #nxh ∗
+     dangle_frag (Some h)) ∗
+    ∃ i r b : nat, ith_read i r (h + 1) ∗ ⌜r ≤ h⌝ ∗ br_lb b ∗
+      (⌜b < r⌝ -∗
+       ith_rp i rs_canceled
+       ∨ ith_rp i rs_aborted ∨ ith_rp i (rs_proc (Some rsp_completed))).
+  Proof using. 
+    iIntros "#HTH CH CFL DFRAG HQ AUTHS Q TAIL DUMMY BR FL DAUTH OHV RHI RH TOK CLOS HEAD HEAD'".
+
+    iMod (dangle_update _ _ (Some h) with "[$] [$]") as "[DAUTH DFRAG]".
+
+    iAssert (|==> auths (h + 1) t br fl ∗ @me_exact _ q_me_h (h + 1))%I with "[CH AUTHS]" as "UPD".
+    { rewrite /auths. iDestruct "AUTHS" as "(AUTH&?&?&?)". iFrame.
+      iApply (me_update with "AUTH CH"). lia. }
+    iMod "UPD" as "[AUTHS CH]".
+
+    iFrame.
+
+    iDestruct (dequeue_restore_QI with "[$] [$] [$] [$] [$] [$]") as "[QI HNI]".
+    all: try by eauto. 
+
+    iDestruct (cancel_rop with "[$]") as "#CNC".
+    { red. rewrite Nat.add_1_r. reflexivity. }
+    
+    iDestruct (take_snapshot with "[$]") as "#SHT".
+    iDestruct "SHT" as "(_&_&#BR_LB&_)". 
+
+    rewrite /read_hist_interp. iDestruct "RHI" as "(ROPA & ROP & RHIST & %RH_WF & #OLDS)". 
+    rewrite /rop_interp.
+    destruct rop as [n| ]. 
+    - iDestruct ("ROP" with "[//]") as "(%r & %rp & READ_ & RP & ROP)".      
+      destruct RH_WF as (n' & DOM & [? | [=]] & RH_WF); [done| ]. subst n'. 
+      iMod (read_hist_wf_bump with "[$] [RP]") as "(%r' & %rp' & RHIST & #READ & %RH_WF' & RP & %READ_BOUND)".
+      { eexists. eauto. }
+      { rewrite DOM dom_max_set_fold. iFrame. }
+      rewrite DOM dom_max_set_fold. 
+      iDestruct (ith_read_agree with "READ READ_") as %<-.
+      iFrame "READ". iFrame "%". iFrame "BR_LB". 
+      rewrite -(bi.sep_True' ( ⌜ _ ⌝ -∗ _ )%I). iApply fupd_frame_l. iSplit.
+      { iIntros (LT). iDestruct "ROP" as "[SAFE | [-> _]]".
+        2: { iFrame. }
+        iDestruct "SAFE" as "[FROM_HEAD | [FROM_DANGLE | FROM_BR]]".
+        - iDestruct "FROM_HEAD" as "[-> [-> | (-> & -> & ?)]]".
+          + simpl. iFrame. 
+          + lia. 
+        - iDestruct "FROM_DANGLE" as "[(-> & -> & %X) ?]".
+          clear -X. by destruct X. 
+        - iDestruct "FROM_BR" as "([-> ->] & -> & ?)". lia. } 
+
+      iClear "HTH".
+      iMod ("CLOS" with "[-]") as "_"; [| done].
+      iFrame "QI AUTHS OHV HQ RH DAUTH TOK RHIST ROPA". iNext.
+      rewrite Nat.add_sub. rewrite HTH /=. 
+      
+      iSplit.
+      { iPureIntro. red. red in ORDER. repeat split; try lia. }
+      iSplitL "HNI". 
+      { iRight. by iFrame. }
+      rewrite DOM dom_max_set_fold in RH_WF'.
+      iFrame "%". 
+      iSplit.
+      2: { iApply old_rps_olds.
+           iDestruct (old_rps_olds with "OLDS") as "foo". 
+           by rewrite delete_insert_delete. }
+      rewrite /rop_interp. iIntros (i_ [=]). subst i_. 
+
+      iFrame "READ_ RP". 
+      iDestruct "ROP" as "[[HEAD | [DANGLE | FL]] | CANCEL_WITNESS]".
+      + iDestruct "HEAD" as "(-> & [-> | (-> & -> & ?)])".
+        * iRight. simpl. by iFrame "#∗".
+        * iLeft. iRight. iLeft. iFrame.
+          iPureIntro. split.
+          ** split; [lia | done].
+          ** simpl. done. 
+      + iDestruct "DANGLE" as "((_ & _ & %) & _)". by destruct H.
+      + iDestruct "FL"as "([-> ->] & -> & ?)". 
+        iLeft. rewrite /safe_read. iFrame. 
+        repeat iRight. iFrame. done.
+      + iDestruct "CANCEL_WITNESS" as "(-> & CW)".
+        iRight. by iFrame.
+    - destruct RH_WF as (n & DOM & [? | [=]] & RH_WF).
+      destruct (hist !! n) as [[[??]?] | ] eqn:NTH. 
+      2: { apply not_elem_of_dom in NTH. rewrite DOM in NTH.
+           rewrite elem_of_set_seq in NTH. lia. }
+      iDestruct (big_sepM_lookup with "OLDS") as "RP".
+      { simpl. apply NTH. } 
+      iDestruct "RP" as "(%rp & RP & %FIN & #LB)".
+      iDestruct (ith_rp_hist_compat with "[$] [$]") as %(? & ? & LE').
+      rewrite NTH in H0. inversion H0. subst x. simpl in *.
+
+      iDestruct (read_hist_get hist n with "RHIST") as "#READ".
+      { rewrite NTH. repeat f_equal. }
+      
+      iMod (read_hist_wf_bump with "[$] [RP]") as "(%r' & %rp' & RHIST & #READ' & %RH_WF' & RP_ & %READ_BOUND)".
+      { eexists. eauto. }
+      { rewrite DOM dom_max_set_fold. iFrame "RP". }
+      rewrite DOM dom_max_set_fold.
+      iDestruct (ith_read_agree with "READ READ'") as %->.
+      iFrame "% READ' BR_LB".
+      rewrite -(bi.sep_True' ( ⌜ _ ⌝ -∗ _ )%I). iApply fupd_frame_l. iSplit.
+      { iIntros (LT). destruct FIN as [-> | [-> | [-> | ->]]].
+        all: try by iFrame.
+        iDestruct "LB" as "[LB | [%RS_AB | %RS_CANC]]".
+        2, 3: done. 
+        iDestruct (br_lb_bound with "[$] [$]") as %?. lia. }
+
+      iMod ("CLOS" with "[-]") as "_"; [| done].
+      iFrame "QI AUTHS OHV HQ RH DAUTH TOK RHIST". iNext.
+      iExists _. rewrite Nat.add_sub. rewrite HTH /=.
+      
+      iSplit.
+      { iPureIntro. red. red in ORDER. repeat split; try lia. }
+      iSplitL "HNI". 
+      { iRight. by iFrame. }
+      rewrite DOM dom_max_set_fold in RH_WF'.
+      destruct RH_WF as (SEQ &  BB). 
+      Unshelve. 2: exact None. 
+      rewrite bi.sep_assoc.
+      iFrame "ROPA". 
+      rewrite /rop_interp. iSplit. 
+      { iIntros (i_ [=]). }
+      iSplitR.
+      2: { (* TODO: make a lemma? *)
+        rewrite /old_rps. simpl.
+        rewrite -insert_delete_insert.         
+        rewrite insert_union_singleton_l big_sepM_union.
+        2: { apply map_disjoint_dom. rewrite dom_insert_L. set_solver. }
+        iSplitL.
+        2: { iApply (big_sepM_subseteq with "[$]"). apply delete_subseteq. }
+        rewrite big_sepM_singleton. iFrame. iFrame "% #".
+        iSplit. 
+        { iPureIntro. by apply upd_rp_fin_pres. }
+        iDestruct "LB" as "[$ | [-> | ->]]".
+        all: simpl; iRight; iPureIntro; tauto. }
+
+      (* TODO: make a lemma *)
+      rewrite /read_hist_wf.
+      iPureIntro. 
+
+      exists n. split; [| split; [| split]]. 
+    + rewrite dom_insert_L. apply mk_is_Some, elem_of_dom in NTH. set_solver.
+    + tauto. 
+    + intros ?????. rewrite !lookup_insert_Some.
+      intros [(? & ?) | (? & ITH) ] [(? & ?) | (? & JTH) ]; subst; simpl in *; try lia.
+      * apply mk_is_Some, elem_of_dom in JTH.
+        rewrite DOM elem_of_union elem_of_set_seq elem_of_singleton in JTH. lia.
+      * eapply SEQ in H1; eauto. done.
+      * eapply SEQ; eauto.
+    + intros ??. rewrite lookup_insert_Some.         
+      intros [(? & ?) | (? & ITH) ]; subst; simpl; try lia.
+      eapply BB in ITH; eauto. simpl in ITH. lia.
+  Qed.
+
+  Lemma get_to_free_post
+  (pbr : loc)
+  (b b1 : nat)
+  ph h fl ndh r i
+  (ndbr1 : Node)
+  (LEb : b ≤ b1)
+  (PTR_EQ : pbr = ph)
+  (pfl : loc)
+  (ndfl : Node)
+  (hq : HistQueue)
+  (t br : nat)
+  (rop : option nat)
+  (hist : read_hist)
+  (ORDER : hq_state_wf (h + 1) t br fl)
+  (HTH : hq !! h = Some (ph, ndh))
+  (NEMPTY : t ≠ h)
+  (T_LEN : t = length hq)
+  (FLTH : hq !! fl = Some (pfl, ndfl)):
+  ith_node h (ph, ndh) -∗
+  ith_read i r (h + 1) -∗
+  br_lb b -∗
+  (⌜b < r⌝ -∗ ith_rp i rs_canceled ∨ ith_rp i rs_aborted ∨ ith_rp i (rs_proc (Some rsp_completed))) -∗
+  br_lb b1 -∗
+  ith_node b1 (ph, ndbr1) -∗
+  ith_node fl (pfl, ndfl) -∗
+  (⌜∃ nd : Node, hq !! fl = Some (ph, nd)⌝ -∗
+                ⌜∃ nd : Node, Some (ph, ndh) = Some (ph, nd)⌝ -∗ False) -∗
+  @me_exact _ (@q_me_h Σ QL) (h + 1) -∗
+  @me_exact _ (@q_me_fl Σ QL) fl -∗
+  simple_queue.Head q_sq ↦{1 / 2} #ndh.2 -∗
+  dangle_frag (Some h) -∗
+  hq_auth hq -∗
+  auths (h + 1) t br fl -∗
+  phys_queue_interp (drop (h + 1) hq) -∗
+  (∃ nbr : HistNode, ⌜hq !! br = Some nbr⌝ ∗
+           simple_queue.BeingRead q_sq ↦ #nbr.1) -∗
+  hn_interp (pfl, ndfl) -∗
+  dangle_auth (Some h) -∗
+  (let '(v, nxt) := ndh in ph ↦ v ∗ (ph +ₗ 1) ↦ #nxt) -∗
+  ohv_interp -∗
+  read_hist_interp hist rop (h + 1) br fl (Some h) -∗
+  ((∃ pt : loc, read_head_resources t br pt None ∗ rop_token)
+         ∨ read_head_token) -∗
+  dequeue_token -∗
+  (▷ (∃ (hq0 : HistQueue) (h0 t0 br0 fl0 : nat)
+                (rop0 od : option nat) (hist0 : read_hist),
+                queue_inv_inner hq0 h0 t0 br0 fl0 rop0 od hist0) ={
+           ⊤ ∖ ↑queue_ns,⊤}=∗ emp) -∗
+  simple_queue.FreeLater q_sq ↦ #ph -∗
+  |={⊤ ∖ ↑queue_ns,⊤}=>
+    ∃ (x : Node) (x0 : nat), (let '(v, nxt) := x in pfl ↦ v ∗ (pfl +ₗ 1) ↦ #nxt) ∗
+      @me_exact _ q_me_h (h + 1) ∗ @me_exact _ q_me_fl x0 ∗ simple_queue.Head q_sq ↦{
+      1 / 2} #ndh.2 ∗ dangle_frag None.
+  Proof using.
+    iIntros "#HTH #READ #BR0 #NO_FL #BR1 #BRTH1 #FLTH #PFL_NEQ_D".
+    iIntros "CH CFL HEAD' DFRAG HQ AUTHS PQI BR HNI_FL DAUTH HNI OHV RHI RH TOK CLOS FL".
+
+    iDestruct "BR" as "(%nbr & %BRTH & BR)".
+    iDestruct (br_lb_bound with "BR1 AUTHS") as %BR1.
+
+    subst pbr.
+    destruct nbr as [pbr nbr].
+
+    iMod (dangle_update _ _ None with "[$] [$]") as "[DAUTH DFRAG]".
+    iAssert (|==> auths (h + 1) t br h ∗ @me_exact _ q_me_fl h)%I with "[CFL AUTHS]" as "UPD".
+    { rewrite /auths. iDestruct "AUTHS" as "(?&?&?&A)". iFrame.
+      iApply (me_update with "A CFL"). red in ORDER. lia. }
+    iMod "UPD" as "[AUTHS CFL]".
+
+    iDestruct (br_lb_bound with "BR0 [$]") as %BR0.
+    iAssert (queue_interp hq (h + 1) t br h)%I
+      with "[PQI BR FL HNI]" as "QI".
+    { iFrame. iSplit; [done| ].
+      iFrame "%". iFrame. }
+
+    rewrite /read_hist_interp. iDestruct "RHI" as "(ROPA & ROP & RHIST & %RH_WF & #OLDS)".
+    rewrite /rop_interp.
+    destruct rop.
+    - iDestruct ("ROP" with "[//]") as "(%r_ & %rp & READ_ & RP & ROP)".
+      iDestruct (ith_read_hist_compat with "[$] READ_") as %(?&? & READ' & _).
+      iDestruct (ith_read_hist_compat with "[$] READ") as %(?&? & READ & BB).
+      iDestruct (hq_auth_lookup with "[$] BRTH1") as %BRTH1.
+      
+      iAssert (dequeue_resources (h + 1) h ndh.2 None)%I with "[CH CFL HEAD' DFRAG]" as "DR".
+      { iFrame.
+        Set Printing Implicit.
+      }
+
+      iMod ("CLOS" with "[-DR HNI_FL]") as "_".
+      { iFrame. iNext. iFrame "OLDS". iFrame (RH_WF).
+        iSplit.
+        { rewrite /hq_state_wf. iPureIntro. red in ORDER. lia. }
+        iSplitR.
+        { by iLeft. }
+        rewrite /rop_interp.
+        iIntros (i' [=]). subst n.
+        iDestruct "ROP" as "[SAFE | $]".
+        2: { iFrame. }
+        iFrame "READ_".
+          
+        destruct (decide (i' = i)).
+        { subst. rewrite {1}/safe_read. rewrite Nat.add_sub.
+          iDestruct "SAFE" as "[FROM_HEAD | [FROM_DANGLE | FROM_BR]]".
+          - iFrame.
+          - iDestruct "FROM_DANGLE" as "((-> & -> & _) & -> & ?)".
+            iFrame "RP".
+            iLeft. rewrite /safe_read. rewrite Nat.add_sub.
+            do 2 iRight. by iFrame.
+          - iDestruct "FROM_BR" as "([-> ->] & -> & ?)".
+            rewrite READ in READ'. inversion READ'. subst r x1 x2.
+            apply Nat.le_lteq in BR0 as [BR0 | ->].
+            { iSpecialize ("NO_FL" with "[//]"). iExFalso.
+              iAssert (∃ rp', ith_rp i rp' ∗ ⌜ rp' = rs_canceled \/ rp' = rs_aborted \/ rp' = (rs_proc (Some rsp_completed))⌝)%I as "(%rp' & RP' & %RP')".
+              { iDestruct "NO_FL" as "[$|[$|$]]"; set_solver. }
+              iDestruct (ith_rp_le with "RP RP'") as %CM.
+              exfalso. clear -RP' CM.
+              inversion CM; destruct RP' as [-> | [-> | ->]]; try done.
+              subst. inversion RSP. by subst. }
+            rename x into bi.
+            red in RH_WF.
+            destruct RH_WF as (n' & DOM & [? | [=]] & SEQ & BB'); [done| ].
+            subst n'.
+            pose proof READ as EQ%BB'. simpl in EQ.
+            assert (bi = h + 1) as -> by lia.  clear BB EQ.
+            assert (b1 = fl) as -> by lia.
+            rewrite BRTH in BRTH1. inversion BRTH1. subst pbr ndbr1.
+            iDestruct ("PFL_NEQ_D" with "[] []") as "?".
+            { eauto. }
+            { eauto. }
+            done. }
+          
+        assert (i < i') as NEW.
+        { red in RH_WF. destruct RH_WF as (n' & DOM & [? | [=]] & RH_WF); [done| ].
+          subst i'.
+          apply mk_is_Some, elem_of_dom in READ. rewrite DOM elem_of_set_seq in READ.
+          lia. }
+        clear n.
+
+        assert (h + 1 <= r_) as READ'_BOUND.
+        { red in RH_WF. destruct RH_WF as (n' & DOM & [? | [=]] & RH_WF); [done| ].
+          apply proj1 in RH_WF. eapply RH_WF in NEW; eauto. simpl in NEW. lia. }
+        rewrite {1}/safe_read.
+        iDestruct "SAFE" as "[FROM_HEAD | [FROM_DANGLE | FROM_BR]]".
+        + iFrame.
+        + iDestruct "FROM_DANGLE" as "[(-> & -> & _) ?]". lia.
+        + iFrame.
+          iDestruct "FROM_BR" as "([% %] & ?)". subst.
+          red in ORDER. lia. }
+      by iFrame.
+    -
+      iAssert (dequeue_resources (h + 1) h ndh.2 None)%I with "[CH CFL HEAD' DFRAG]" as "DR".
+      { iFrame. }
+
+      iMod ("CLOS" with "[-DR HNI_FL]") as "_".
+      { iFrame. iNext. iFrame "OLDS". iFrame (RH_WF). iSplit.
+        { rewrite /hq_state_wf. iPureIntro. red in ORDER. lia. }
+        iSplitR.
+        { by iLeft. }
+        rewrite /rop_interp. by iIntros (??). }
+      by iFrame.
+  Qed.
+
+  Lemma check_BR_post
+  (h fl : nat) (ph : loc) (ndh : Node) (i r b0 : nat)
+  (READ_BOUND : r ≤ h) (hq : HistQueue) (t br : nat)
+  (rop : option nat) (hist : read_hist)
+  (ORDER : hq_state_wf (h + 1) t br fl)
+  (HTH : hq !! h = Some (ph, ndh))
+  (NEMPTY : t ≠ h)
+  (T_LEN : t = length hq)
+  (pbr : loc)
+  (nbr : Node)
+  (BRTH : hq !! br = Some (pbr, nbr)):    
+  ith_read i r (h + 1) -∗
+  br_lb b0 -∗
+  dangle_frag (Some h) -∗
+  hq_auth hq -∗
+  auths (h + 1) t br fl -∗
+  phys_queue_interp (drop (h + 1) hq) -∗
+  (∃ nfl : HistNode, ⌜hq !! fl = Some nfl⌝ ∗ FreeLater q_sq ↦ #nfl.1 ∗
+           hn_interp nfl) -∗
+  dangle_auth (Some h) -∗
+  (let '(v, nxt) := ndh in ph ↦ v ∗ (ph +ₗ 1) ↦ #nxt) -∗
+  ohv_interp -∗
+  read_hist_interp hist rop (h + 1) br fl (Some h) -∗
+  ((∃ pt : loc, read_head_resources t br pt None ∗ rop_token)
+         ∨ read_head_token) -∗
+  dequeue_token -∗
+  (▷ (∃ (hq0 : HistQueue) (h0 t0 br0 fl0 : nat) 
+                (rop0 od : option nat) (hist0 : read_hist),
+                queue_inv_inner hq0 h0 t0 br0 fl0 rop0 od hist0) ={
+           ⊤ ∖ ↑queue_ns,⊤}=∗ emp) -∗
+  BeingRead q_sq ↦ #(pbr, nbr)%core.1 -∗
+  |={⊤ ∖ ↑queue_ns,⊤}=>
+    dangle_frag (if decide ((pbr, nbr).1 = ph) then Some h else None) ∗
+    (⌜(pbr, nbr).1 = ph⌝ ∨ ⌜(pbr, nbr).1 ≠ ph⌝ ∗
+     (let '(v, nxt) := ndh in ph ↦ v ∗ (ph +ₗ 1) ↦ #nxt)) ∗
+    ∃ (b' : nat) (ndbr' : Node), br_lb b' ∗ ⌜b0 ≤ b'⌝ ∗
+      ith_node b' ((pbr, nbr).1, ndbr').
+  Proof using. 
+    iIntros "#READ #BR0 DFRAG HQ AUTHS PQI FL DAUTH HNI OHV RHI RH TOK CLOS BR".
+    iDestruct (br_lb_bound with "BR0 AUTHS") as %BR0. 
+    iDestruct (take_snapshot with "[$]") as "#SHT".
+    iDestruct (hq_auth_get_ith with "HQ") as "#BRTH'".
+    { apply BRTH. }
+    iFrame "BRTH'". 
+
+    iAssert (queue_interp hq (h + 1) t br fl)%I with "[PQI BR FL]" as "QI".
+    { by iFrame. }
+    iAssert (br_lb br ∗ ⌜b0 ≤ br⌝)%I as "$".
+    { iSplit; [| done].
+      iDestruct "SHT" as "(?&?&?&?)". done. }
+
+    simpl.
+    destruct (decide (pbr = ph)) as [-> | NEQ].
+    -
+      iFrame. 
+      iMod ("CLOS" with "[-]") as "_".
+      { iFrame "#∗ %". iNext.
+        rewrite Nat.add_sub HTH /=.
+        iRight. by iFrame. }
+      iModIntro. by iLeft.
+    - rewrite /read_hist_interp. iDestruct "RHI" as "(ROPA & ROP & RHIST & %RH_WF & #OLDS)".  
+      iDestruct (ith_read_hist_compat with "[$] [$]") as %(b & p & READ & INCR_BOUND). 
+      iMod (dangle_update _ _ None with "[$] [$]") as "[DAUTH DFRAG]".
+      iFrame.      
+      iApply fupd_or. iRight. iFrame "HNI".
+      rewrite -(bi.sep_True' ⌜ _ ≠ _ ⌝%I). iApply fupd_frame_l. iSplit; [done| ].
+      iMod ("CLOS" with "[-]") as "_"; [| done]. 
+
+      rewrite /rop_interp.
+      destruct rop.
+      2: { iFrame "#∗ %". iNext. iSplitR.
+           { by iLeft. }
+           rewrite /rop_interp. by iIntros (??). }
+      
+      iDestruct ("ROP" with "[//]") as "(%r_ & %rp & READ_ & RP & ROP)".
+      iDestruct (ith_read_hist_compat with "[$] READ_") as %(?&? & READ' & _). 
+
+      iFrame. iFrame "OLDS".
+      iNext. iFrame (RH_WF ORDER). iSplitR.
+      { by iLeft. }
+      rewrite /rop_interp.
+      iIntros (i' [=]). subst n.
+      iDestruct "ROP" as "[SAFE | $]".
+      2: { iFrame "#∗". }
+
+      destruct (decide (i' = i)). 
+      { subst. rewrite {1}/safe_read. rewrite Nat.add_sub.
+        iFrame "READ_". 
+        iDestruct "SAFE" as "[FROM_HEAD | [FROM_DANGLE | FROM_BR]]".
+        - iFrame.
+        - iDestruct "FROM_DANGLE" as "[(-> & -> & _) ?]".
+          congruence.
+        - iFrame. }
+
+      assert (i < i') as NEW.
+      { red in RH_WF. destruct RH_WF as (n' & DOM & [? | [=]] & RH_WF); [done| ].
+        subst i'.
+        apply mk_is_Some, elem_of_dom in READ. rewrite DOM elem_of_set_seq in READ.
+        lia. }
+      clear n.
+      
+      assert (h + 1 <= r_) as READ'_BOUND.
+      { red in RH_WF. destruct RH_WF as (n' & DOM & [? | [=]] & RH_WF); [done| ].
+        subst. 
+        apply proj1 in RH_WF. eapply RH_WF in NEW; eauto. simpl in NEW. lia. }
+      iFrame "READ_".
+      rewrite {1}/safe_read.
+      iDestruct "SAFE" as "[FROM_HEAD | [FROM_DANGLE | FROM_BR]]".
+      + iFrame.
+      + iDestruct "FROM_DANGLE" as "[(-> & -> & _) ?]". lia.
+      + iFrame.
+  Qed. 
+
+End DequeueGhost.
